Lib.v
@@ -24,6 +24,46 @@ Generalizable All Variables.
 
 (** The following are extensions to the Coq standard library. *)
 
+Ltac move_to_top x :=
+  match reverse goal with
+  | H : _ |- _ => try move x after H
+  end.
+
+Tactic Notation "assert_eq" ident(x) constr(v) :=
+  let H := fresh in
+  assert (x = v) as H by reflexivity;
+  clear H.
+
+Tactic Notation "Case_aux" ident(x) constr(name) :=
+  first [
+    set (x := name); move_to_top x
+  | assert_eq x name; move_to_top x
+  | fail 1 "because we are working on a different case" ].
+
+Tactic Notation "Case" constr(name) := Case_aux Case name.
+Tactic Notation "SCase" constr(name) := Case_aux SCase name.
+Tactic Notation "SSCase" constr(name) := Case_aux SSCase name.
+Tactic Notation "SSSCase" constr(name) := Case_aux SSSCase name.
+Tactic Notation "SSSSCase" constr(name) := Case_aux SSSSCase name.
+Tactic Notation "SSSSSCase" constr(name) := Case_aux SSSSSCase name.
+Tactic Notation "SSSSSSCase" constr(name) := Case_aux SSSSSSCase name.
+Tactic Notation "SSSSSSSCase" constr(name) := Case_aux SSSSSSSCase name.
+
+Require String.
+Open Scope string_scope.
+
+Definition existT_in_cons : forall {A a} {l : list A},
+  {x : A & In x l} -> {x : A & In x (a :: l)}.
+Proof.
+  destruct l; intros; simpl.
+    destruct X. inversion i.
+  destruct X. exists x.
+  apply in_inv in i.
+  destruct i.
+    right. left. assumption.
+  right. right. assumption.
+Defined.
+
 (** ** option *)
 
 Fixpoint catMaybes {a : Set} (l : list (option a)) : list a :=
